First version of external core models.

hax-lib/proof-libs/fstar/core/Core_models.Bundle.fst
@@ -3,10 +3,12 @@ module Core_models.Bundle
 open FStar.Mul
 open Rust_primitives
 
+/// See [`std::option::Option`]
 type t_Option (v_T: Type0) =
   | Option_Some : v_T -> t_Option v_T
   | Option_None : t_Option v_T
 
+/// See [`std::option::Option::is_some_and`]
 let impl__is_some_and
       (#v_T #v_F: Type0)
       (#[FStar.Tactics.Typeclasses.tcresolve ()] i0: Core_models.Ops.Function.t_FnOnce v_F v_T)
@@ -17,8 +19,9 @@ let impl__is_some_and
   match self <: t_Option v_T with
   | Option_None  -> false
   | Option_Some x ->
-    Core_models.Ops.Function.f_call_once #v_F #v_T #FStar.Tactics.Typeclasses.solve f x
+    Core_models.Ops.Function.f_call_once #v_F #v_T #FStar.Tactics.Typeclasses.solve f (x <: v_T)
 
+/// See [`std::option::Option::is_none_or`]
 let impl__is_none_or
       (#v_T #v_F: Type0)
       (#[FStar.Tactics.Typeclasses.tcresolve ()] i0: Core_models.Ops.Function.t_FnOnce v_F v_T)
@@ -29,18 +32,21 @@ let impl__is_none_or
   match self <: t_Option v_T with
   | Option_None  -> true
   | Option_Some x ->
-    Core_models.Ops.Function.f_call_once #v_F #v_T #FStar.Tactics.Typeclasses.solve f x
+    Core_models.Ops.Function.f_call_once #v_F #v_T #FStar.Tactics.Typeclasses.solve f (x <: v_T)
 
+/// See [`std::option::Option::as_ref`]
 let impl__as_ref (#v_T: Type0) (self: t_Option v_T) : t_Option v_T =
   match self <: t_Option v_T with
   | Option_Some x -> Option_Some x <: t_Option v_T
   | Option_None  -> Option_None <: t_Option v_T
 
+/// See [`std::option::Option::unwrap_or`]
 let impl__unwrap_or (#v_T: Type0) (self: t_Option v_T) (v_default: v_T) : v_T =
   match self <: t_Option v_T with
   | Option_Some x -> x
   | Option_None  -> v_default
 
+/// See [`std::option::Option::unwrap_or_else`]
 let impl__unwrap_or_else
       (#v_T #v_F: Type0)
       (#[FStar.Tactics.Typeclasses.tcresolve ()]
@@ -59,6 +65,7 @@ let impl__unwrap_or_else
       f
       (() <: Prims.unit)
 
+/// See [`std::option::Option::unwrap_or_default`]
 let impl__unwrap_or_default
       (#v_T: Type0)
       (#[FStar.Tactics.Typeclasses.tcresolve ()] i0: Core_models.Default.t_Default v_T)
@@ -68,6 +75,7 @@ let impl__unwrap_or_default
   | Option_Some x -> x
   | Option_None  -> Core_models.Default.f_default #v_T #FStar.Tactics.Typeclasses.solve ()
 
+/// See [`std::option::Option::map`]
 let impl__map
       (#v_T #v_U #v_F: Type0)
       (#[FStar.Tactics.Typeclasses.tcresolve ()] i0: Core_models.Ops.Function.t_FnOnce v_F v_T)
@@ -78,11 +86,12 @@ let impl__map
   match self <: t_Option v_T with
   | Option_Some x ->
     Option_Some
-    (Core_models.Ops.Function.f_call_once #v_F #v_T #FStar.Tactics.Typeclasses.solve f x)
+    (Core_models.Ops.Function.f_call_once #v_F #v_T #FStar.Tactics.Typeclasses.solve f (x <: v_T))
     <:
     t_Option v_U
   | Option_None  -> Option_None <: t_Option v_U
 
+/// See [`std::option::Option::map_or`]
 let impl__map_or
       (#v_T #v_U #v_F: Type0)
       (#[FStar.Tactics.Typeclasses.tcresolve ()] i0: Core_models.Ops.Function.t_FnOnce v_F v_T)
@@ -93,9 +102,10 @@ let impl__map_or
     : v_U =
   match self <: t_Option v_T with
   | Option_Some t ->
-    Core_models.Ops.Function.f_call_once #v_F #v_T #FStar.Tactics.Typeclasses.solve f t
+    Core_models.Ops.Function.f_call_once #v_F #v_T #FStar.Tactics.Typeclasses.solve f (t <: v_T)
   | Option_None  -> v_default
 
+/// See [`std::option::Option::map_or_else`]
 let impl__map_or_else
       (#v_T #v_U #v_D #v_F: Type0)
       (#[FStar.Tactics.Typeclasses.tcresolve ()] i0: Core_models.Ops.Function.t_FnOnce v_F v_T)
@@ -110,7 +120,7 @@ let impl__map_or_else
     : v_U =
   match self <: t_Option v_T with
   | Option_Some t ->
-    Core_models.Ops.Function.f_call_once #v_F #v_T #FStar.Tactics.Typeclasses.solve f t
+    Core_models.Ops.Function.f_call_once #v_F #v_T #FStar.Tactics.Typeclasses.solve f (t <: v_T)
   | Option_None  ->
     Core_models.Ops.Function.f_call_once #v_D
       #Prims.unit
@@ -118,6 +128,7 @@ let impl__map_or_else
       v_default
       (() <: Prims.unit)
 
+/// See [`std::option::Option::map_or_default`]
 let impl__map_or_default
       (#v_T #v_U #v_F: Type0)
       (#[FStar.Tactics.Typeclasses.tcresolve ()] i0: Core_models.Ops.Function.t_FnOnce v_F v_T)
@@ -128,9 +139,10 @@ let impl__map_or_default
     : v_U =
   match self <: t_Option v_T with
   | Option_Some t ->
-    Core_models.Ops.Function.f_call_once #v_F #v_T #FStar.Tactics.Typeclasses.solve f t
+    Core_models.Ops.Function.f_call_once #v_F #v_T #FStar.Tactics.Typeclasses.solve f (t <: v_T)
   | Option_None  -> Core_models.Default.f_default #v_U #FStar.Tactics.Typeclasses.solve ()
 
+/// See [`std::option::Option::and_then`]
 let impl__and_then
       (#v_T #v_U #v_F: Type0)
       (#[FStar.Tactics.Typeclasses.tcresolve ()] i0: Core_models.Ops.Function.t_FnOnce v_F v_T)
@@ -140,12 +152,91 @@ let impl__and_then
     : t_Option v_U =
   match self <: t_Option v_T with
   | Option_Some x ->
-    Core_models.Ops.Function.f_call_once #v_F #v_T #FStar.Tactics.Typeclasses.solve f x
+    Core_models.Ops.Function.f_call_once #v_F #v_T #FStar.Tactics.Typeclasses.solve f (x <: v_T)
   | Option_None  -> Option_None <: t_Option v_U
 
+/// See [`std::option::Option::take`]
+/// Note: The interface in Rust is wrong, but is good after extraction.
+/// We cannot make a useful model with the right interface so we lose the executability.
 let impl__take (#v_T: Type0) (self: t_Option v_T) : (t_Option v_T & t_Option v_T) =
   (Option_None <: t_Option v_T), self <: (t_Option v_T & t_Option v_T)
 
+/// See [`std::option::Option::filter`]
+assume
+val impl__filter':
+    #v_T: Type0 ->
+    #v_P: Type0 ->
+    {| i0: Core_models.Ops.Function.t_FnOnce v_P v_T |} ->
+    #_: unit{i0.Core_models.Ops.Function.f_Output == bool} ->
+    self: t_Option v_T ->
+    predicate: v_P
+  -> t_Option v_T
+
+unfold
+let impl__filter
+      (#v_T #v_P: Type0)
+      (#[FStar.Tactics.Typeclasses.tcresolve ()] i0: Core_models.Ops.Function.t_FnOnce v_P v_T)
+      (#_: unit{i0.Core_models.Ops.Function.f_Output == bool})
+     = impl__filter' #v_T #v_P #i0 #_
+
+/// See [`std::option::Option::or`]
+let impl__or (#v_T: Type0) (self optb: t_Option v_T) : t_Option v_T =
+  match self <: t_Option v_T with
+  | Option_Some x -> Option_Some x <: t_Option v_T
+  | Option_None  -> optb
+
+/// See [`std::option::Option::or_else`]
+let impl__or_else
+      (#v_T #v_F: Type0)
+      (#[FStar.Tactics.Typeclasses.tcresolve ()]
+          i0:
+          Core_models.Ops.Function.t_FnOnce v_F Prims.unit)
+      (#_: unit{i0.Core_models.Ops.Function.f_Output == t_Option v_T})
+      (self: t_Option v_T)
+      (f: v_F)
+    : t_Option v_T =
+  match self <: t_Option v_T with
+  | Option_Some x -> Option_Some x <: t_Option v_T
+  | Option_None  ->
+    Core_models.Ops.Function.f_call_once #v_F
+      #Prims.unit
+      #FStar.Tactics.Typeclasses.solve
+      f
+      (() <: Prims.unit)
+
+/// See [`std::option::Option::xor`]
+let impl__xor (#v_T: Type0) (self optb: t_Option v_T) : t_Option v_T =
+  match self, optb <: (t_Option v_T & t_Option v_T) with
+  | Option_Some a, Option_None  -> Option_Some a <: t_Option v_T
+  | Option_None , Option_Some b -> Option_Some b <: t_Option v_T
+  | _ -> Option_None <: t_Option v_T
+
+/// See [`std::option::Option::zip`]
+let impl__zip (#v_T #v_U: Type0) (self: t_Option v_T) (other: t_Option v_U) : t_Option (v_T & v_U) =
+  match self, other <: (t_Option v_T & t_Option v_U) with
+  | Option_Some a, Option_Some b -> Option_Some (a, b <: (v_T & v_U)) <: t_Option (v_T & v_U)
+  | _ -> Option_None <: t_Option (v_T & v_U)
+
+/// See [`std::option::Option::inspect`]
+let impl__inspect
+      (#v_T #v_F: Type0)
+      (#[FStar.Tactics.Typeclasses.tcresolve ()] i0: Core_models.Ops.Function.t_FnOnce v_F v_T)
+      (#_: unit{i0.Core_models.Ops.Function.f_Output == Prims.unit})
+      (self: t_Option v_T)
+      (f: v_F)
+    : t_Option v_T =
+  let _:Prims.unit =
+    match self <: t_Option v_T with
+    | Option_Some x ->
+      let _:Prims.unit =
+        Core_models.Ops.Function.f_call_once #v_F #v_T #FStar.Tactics.Typeclasses.solve f (x <: v_T)
+      in
+      ()
+    | _ -> ()
+  in
+  self
+
+/// See [`std::option::Option::is_some`]
 let impl__is_some (#v_T: Type0) (self: t_Option v_T)
     : Prims.Pure bool
       Prims.l_True
@@ -157,30 +248,50 @@ let impl__is_some (#v_T: Type0) (self: t_Option v_T)
   | Option_Some _ -> true
   | _ -> false
 
+/// See [`std::option::Option::is_none`]
 let impl__is_none (#v_T: Type0) (self: t_Option v_T) : bool =
   (impl__is_some #v_T self <: bool) =. false
 
+/// See [`std::option::Option::expect`]
 let impl__expect (#v_T: Type0) (self: t_Option v_T) (e_msg: string)
     : Prims.Pure v_T (requires impl__is_some #v_T self) (fun _ -> Prims.l_True) =
   match self <: t_Option v_T with
   | Option_Some v_val -> v_val
   | Option_None  -> Core_models.Panicking.Internal.panic #v_T ()
 
+/// See [`std::option::Option::unwrap`]
 let impl__unwrap (#v_T: Type0) (self: t_Option v_T)
     : Prims.Pure v_T (requires impl__is_some #v_T self) (fun _ -> Prims.l_True) =
   match self <: t_Option v_T with
   | Option_Some v_val -> v_val
   | Option_None  -> Core_models.Panicking.Internal.panic #v_T ()
 
+/// See [`std::option::Option::flatten`]
+let impl_1__flatten (#v_T: Type0) (self: t_Option (t_Option v_T)) : t_Option v_T =
+  match self <: t_Option (t_Option v_T) with
+  | Option_Some inner -> inner
+  | Option_None  -> Option_None <: t_Option v_T
+
+[@@ FStar.Tactics.Typeclasses.tcinstance]
+let impl_2 (#v_T: Type0) : Core_models.Default.t_Default (t_Option v_T) =
+  {
+    f_default_pre = (fun (_: Prims.unit) -> true);
+    f_default_post = (fun (_: Prims.unit) (out: t_Option v_T) -> true);
+    f_default = fun (_: Prims.unit) -> Option_None <: t_Option v_T
+  }
+
+/// See [`std::result::Result`]
 type t_Result (v_T: Type0) (v_E: Type0) =
   | Result_Ok : v_T -> t_Result v_T v_E
   | Result_Err : v_E -> t_Result v_T v_E
 
+/// See [`std::option::Option::ok_or`]
 let impl__ok_or (#v_T #v_E: Type0) (self: t_Option v_T) (err: v_E) : t_Result v_T v_E =
   match self <: t_Option v_T with
   | Option_Some v -> Result_Ok v <: t_Result v_T v_E
   | Option_None  -> Result_Err err <: t_Result v_T v_E
 
+/// See [`std::option::Option::ok_or_else`]
 let impl__ok_or_else
       (#v_T #v_E #v_F: Type0)
       (#[FStar.Tactics.Typeclasses.tcresolve ()]
@@ -202,11 +313,78 @@ let impl__ok_or_else
     <:
     t_Result v_T v_E
 
+/// See [`std::result::Result::is_ok`]
+let impl__is_ok (#v_T #v_E: Type0) (self: t_Result v_T v_E) : bool =
+  match self <: t_Result v_T v_E with
+  | Result_Ok _ -> true
+  | _ -> false
+
+/// See [`std::result::Result::is_ok_and`]
+let impl__is_ok_and
+      (#v_T #v_E #v_F: Type0)
+      (#[FStar.Tactics.Typeclasses.tcresolve ()] i0: Core_models.Ops.Function.t_FnOnce v_F v_T)
+      (#_: unit{i0.Core_models.Ops.Function.f_Output == bool})
+      (self: t_Result v_T v_E)
+      (f: v_F)
+    : bool =
+  match self <: t_Result v_T v_E with
+  | Result_Ok t ->
+    Core_models.Ops.Function.f_call_once #v_F #v_T #FStar.Tactics.Typeclasses.solve f (t <: v_T)
+  | Result_Err _ -> false
+
+/// See [`std::result::Result::is_err`]
+let impl__is_err (#v_T #v_E: Type0) (self: t_Result v_T v_E) : bool =
+  ~.(impl__is_ok #v_T #v_E self <: bool)
+
+/// See [`std::result::Result::is_err_and`]
+let impl__is_err_and
+      (#v_T #v_E #v_F: Type0)
+      (#[FStar.Tactics.Typeclasses.tcresolve ()] i0: Core_models.Ops.Function.t_FnOnce v_F v_E)
+      (#_: unit{i0.Core_models.Ops.Function.f_Output == bool})
+      (self: t_Result v_T v_E)
+      (f: v_F)
+    : bool =
+  match self <: t_Result v_T v_E with
+  | Result_Ok _ -> false
+  | Result_Err e ->
+    Core_models.Ops.Function.f_call_once #v_F #v_E #FStar.Tactics.Typeclasses.solve f (e <: v_E)
+
+/// See [`std::result::Result::as_ref`]
+let impl__as_ref__from__result (#v_T #v_E: Type0) (self: t_Result v_T v_E) : t_Result v_T v_E =
+  match self <: t_Result v_T v_E with
+  | Result_Ok t -> Result_Ok t <: t_Result v_T v_E
+  | Result_Err e -> Result_Err e <: t_Result v_T v_E
+
+/// See [`std::result::Result::unwrap_or`]
 let impl__unwrap_or__from__result (#v_T #v_E: Type0) (self: t_Result v_T v_E) (v_default: v_T) : v_T =
   match self <: t_Result v_T v_E with
   | Result_Ok t -> t
   | Result_Err _ -> v_default
 
+/// See [`std::result::Result::unwrap_or_else`]
+let impl__unwrap_or_else__from__result
+      (#v_T #v_E #v_F: Type0)
+      (#[FStar.Tactics.Typeclasses.tcresolve ()] i0: Core_models.Ops.Function.t_FnOnce v_F v_E)
+      (#_: unit{i0.Core_models.Ops.Function.f_Output == v_T})
+      (self: t_Result v_T v_E)
+      (op: v_F)
+    : v_T =
+  match self <: t_Result v_T v_E with
+  | Result_Ok t -> t
+  | Result_Err e ->
+    Core_models.Ops.Function.f_call_once #v_F #v_E #FStar.Tactics.Typeclasses.solve op (e <: v_E)
+
+/// See [`std::result::Result::unwrap_or_default`]
+let impl__unwrap_or_default__from__result
+      (#v_T #v_E: Type0)
+      (#[FStar.Tactics.Typeclasses.tcresolve ()] i0: Core_models.Default.t_Default v_T)
+      (self: t_Result v_T v_E)
+    : v_T =
+  match self <: t_Result v_T v_E with
+  | Result_Ok t -> t
+  | Result_Err _ -> Core_models.Default.f_default #v_T #FStar.Tactics.Typeclasses.solve ()
+
+/// See [`std::result::Result::map`]
 let impl__map__from__result
       (#v_T #v_E #v_U #v_F: Type0)
       (#[FStar.Tactics.Typeclasses.tcresolve ()] i0: Core_models.Ops.Function.t_FnOnce v_F v_T)
@@ -216,11 +394,13 @@ let impl__map__from__result
     : t_Result v_U v_E =
   match self <: t_Result v_T v_E with
   | Result_Ok t ->
-    Result_Ok (Core_models.Ops.Function.f_call_once #v_F #v_T #FStar.Tactics.Typeclasses.solve op t)
+    Result_Ok
+    (Core_models.Ops.Function.f_call_once #v_F #v_T #FStar.Tactics.Typeclasses.solve op (t <: v_T))
     <:
     t_Result v_U v_E
   | Result_Err e -> Result_Err e <: t_Result v_U v_E
 
+/// See [`std::result::Result::map_or`]
 let impl__map_or__from__result
       (#v_T #v_E #v_U #v_F: Type0)
       (#[FStar.Tactics.Typeclasses.tcresolve ()] i0: Core_models.Ops.Function.t_FnOnce v_F v_T)
@@ -231,9 +411,10 @@ let impl__map_or__from__result
     : v_U =
   match self <: t_Result v_T v_E with
   | Result_Ok t ->
-    Core_models.Ops.Function.f_call_once #v_F #v_T #FStar.Tactics.Typeclasses.solve f t
-  | Result_Err e_e -> v_default
+    Core_models.Ops.Function.f_call_once #v_F #v_T #FStar.Tactics.Typeclasses.solve f (t <: v_T)
+  | Result_Err _ -> v_default
 
+/// See [`std::result::Result::map_or_else`]
 let impl__map_or_else__from__result
       (#v_T #v_E #v_U #v_D #v_F: Type0)
       (#[FStar.Tactics.Typeclasses.tcresolve ()] i0: Core_models.Ops.Function.t_FnOnce v_F v_T)
@@ -246,10 +427,29 @@ let impl__map_or_else__from__result
     : v_U =
   match self <: t_Result v_T v_E with
   | Result_Ok t ->
-    Core_models.Ops.Function.f_call_once #v_F #v_T #FStar.Tactics.Typeclasses.solve f t
+    Core_models.Ops.Function.f_call_once #v_F #v_T #FStar.Tactics.Typeclasses.solve f (t <: v_T)
   | Result_Err e ->
-    Core_models.Ops.Function.f_call_once #v_D #v_E #FStar.Tactics.Typeclasses.solve v_default e
+    Core_models.Ops.Function.f_call_once #v_D
+      #v_E
+      #FStar.Tactics.Typeclasses.solve
+      v_default
+      (e <: v_E)
 
+/// See [`std::result::Result::map_or_default`]
+let impl__map_or_default__from__result
+      (#v_T #v_E #v_U #v_F: Type0)
+      (#[FStar.Tactics.Typeclasses.tcresolve ()] i0: Core_models.Ops.Function.t_FnOnce v_F v_T)
+      (#[FStar.Tactics.Typeclasses.tcresolve ()] i1: Core_models.Default.t_Default v_U)
+      (#_: unit{i0.Core_models.Ops.Function.f_Output == v_U})
+      (self: t_Result v_T v_E)
+      (f: v_F)
+    : v_U =
+  match self <: t_Result v_T v_E with
+  | Result_Ok t ->
+    Core_models.Ops.Function.f_call_once #v_F #v_T #FStar.Tactics.Typeclasses.solve f (t <: v_T)
+  | Result_Err _ -> Core_models.Default.f_default #v_U #FStar.Tactics.Typeclasses.solve ()
+
+/// See [`std::result::Result::map_err`]
 let impl__map_err
       (#v_T #v_E #v_F #v_O: Type0)
       (#[FStar.Tactics.Typeclasses.tcresolve ()] i0: Core_models.Ops.Function.t_FnOnce v_O v_E)
@@ -261,15 +461,68 @@ let impl__map_err
   | Result_Ok t -> Result_Ok t <: t_Result v_T v_F
   | Result_Err e ->
     Result_Err
-    (Core_models.Ops.Function.f_call_once #v_O #v_E #FStar.Tactics.Typeclasses.solve op e)
+    (Core_models.Ops.Function.f_call_once #v_O #v_E #FStar.Tactics.Typeclasses.solve op (e <: v_E))
     <:
     t_Result v_T v_F
 
-let impl__is_ok (#v_T #v_E: Type0) (self: t_Result v_T v_E) : bool =
-  match self <: t_Result v_T v_E with
-  | Result_Ok _ -> true
-  | _ -> false
+/// See [`std::result::Result::inspect`]
+let impl__inspect__from__result
+      (#v_T #v_E #v_F: Type0)
+      (#[FStar.Tactics.Typeclasses.tcresolve ()] i0: Core_models.Ops.Function.t_FnOnce v_F v_T)
+      (#_: unit{i0.Core_models.Ops.Function.f_Output == Prims.unit})
+      (self: t_Result v_T v_E)
+      (f: v_F)
+    : t_Result v_T v_E =
+  let _:Prims.unit =
+    match self <: t_Result v_T v_E with
+    | Result_Ok t ->
+      let _:Prims.unit =
+        Core_models.Ops.Function.f_call_once #v_F #v_T #FStar.Tactics.Typeclasses.solve f (t <: v_T)
+      in
+      ()
+    | _ -> ()
+  in
+  self
 
+/// See [`std::result::Result::inspect_err`]
+let impl__inspect_err
+      (#v_T #v_E #v_F: Type0)
+      (#[FStar.Tactics.Typeclasses.tcresolve ()] i0: Core_models.Ops.Function.t_FnOnce v_F v_E)
+      (#_: unit{i0.Core_models.Ops.Function.f_Output == Prims.unit})
+      (self: t_Result v_T v_E)
+      (f: v_F)
+    : t_Result v_T v_E =
+  let _:Prims.unit =
+    match self <: t_Result v_T v_E with
+    | Result_Err e ->
+      let _:Prims.unit =
+        Core_models.Ops.Function.f_call_once #v_F #v_E #FStar.Tactics.Typeclasses.solve f (e <: v_E)
+      in
+      ()
+    | _ -> ()
+  in
+  self
+
+/// See [`std::result::Result::ok`]
+let impl__ok (#v_T #v_E: Type0) (self: t_Result v_T v_E) : t_Option v_T =
+  match self <: t_Result v_T v_E with
+  | Result_Ok x -> Option_Some x <: t_Option v_T
+  | Result_Err _ -> Option_None <: t_Option v_T
+
+/// See [`std::result::Result::err`]
+let impl__err (#v_T #v_E: Type0) (self: t_Result v_T v_E) : t_Option v_E =
+  match self <: t_Result v_T v_E with
+  | Result_Ok _ -> Option_None <: t_Option v_E
+  | Result_Err e -> Option_Some e <: t_Option v_E
+
+/// See [`std::result::Result::and`]
+let impl__and (#v_T #v_E #v_U: Type0) (self: t_Result v_T v_E) (res: t_Result v_U v_E)
+    : t_Result v_U v_E =
+  match self <: t_Result v_T v_E with
+  | Result_Ok _ -> res
+  | Result_Err e -> Result_Err e <: t_Result v_U v_E
+
+/// See [`std::result::Result::and_then`]
 let impl__and_then__from__result
       (#v_T #v_E #v_U #v_F: Type0)
       (#[FStar.Tactics.Typeclasses.tcresolve ()] i0: Core_models.Ops.Function.t_FnOnce v_F v_T)
@@ -279,22 +532,81 @@ let impl__and_then__from__result
     : t_Result v_U v_E =
   match self <: t_Result v_T v_E with
   | Result_Ok t ->
-    Core_models.Ops.Function.f_call_once #v_F #v_T #FStar.Tactics.Typeclasses.solve op t
+    Core_models.Ops.Function.f_call_once #v_F #v_T #FStar.Tactics.Typeclasses.solve op (t <: v_T)
   | Result_Err e -> Result_Err e <: t_Result v_U v_E
 
-let impl__ok (#v_T #v_E: Type0) (self: t_Result v_T v_E) : t_Option v_T =
+/// See [`std::result::Result::or`]
+let impl__or__from__result (#v_T #v_E #v_F: Type0) (self: t_Result v_T v_E) (res: t_Result v_T v_F)
+    : t_Result v_T v_F =
   match self <: t_Result v_T v_E with
-  | Result_Ok x -> Option_Some x <: t_Option v_T
-  | Result_Err _ -> Option_None <: t_Option v_T
+  | Result_Ok t -> Result_Ok t <: t_Result v_T v_F
+  | Result_Err _ -> res
 
+/// See [`std::result::Result::or_else`]
+let impl__or_else__from__result
+      (#v_T #v_E #v_F #v_O: Type0)
+      (#[FStar.Tactics.Typeclasses.tcresolve ()] i0: Core_models.Ops.Function.t_FnOnce v_O v_E)
+      (#_: unit{i0.Core_models.Ops.Function.f_Output == t_Result v_T v_F})
+      (self: t_Result v_T v_E)
+      (op: v_O)
+    : t_Result v_T v_F =
+  match self <: t_Result v_T v_E with
+  | Result_Ok t -> Result_Ok t <: t_Result v_T v_F
+  | Result_Err e ->
+    Core_models.Ops.Function.f_call_once #v_O #v_E #FStar.Tactics.Typeclasses.solve op (e <: v_E)
+
+/// See [`std::result::Result::expect`]
+let impl__expect__from__result (#v_T #v_E: Type0) (self: t_Result v_T v_E) (e_msg: string)
+    : Prims.Pure v_T (requires impl__is_ok #v_T #v_E self) (fun _ -> Prims.l_True) =
+  match self <: t_Result v_T v_E with
+  | Result_Ok t -> t
+  | Result_Err _ -> Core_models.Panicking.Internal.panic #v_T ()
+
+/// See [`std::result::Result::unwrap`]
 let impl__unwrap__from__result (#v_T #v_E: Type0) (self: t_Result v_T v_E)
     : Prims.Pure v_T (requires impl__is_ok #v_T #v_E self) (fun _ -> Prims.l_True) =
   match self <: t_Result v_T v_E with
   | Result_Ok t -> t
   | Result_Err _ -> Core_models.Panicking.Internal.panic #v_T ()
 
-let impl__expect__from__result (#v_T #v_E: Type0) (self: t_Result v_T v_E) (e_msg: string)
-    : Prims.Pure v_T (requires impl__is_ok #v_T #v_E self) (fun _ -> Prims.l_True) =
+/// See [`std::result::Result::expect_err`]
+let impl__expect_err (#v_T #v_E: Type0) (self: t_Result v_T v_E) (e_msg: string)
+    : Prims.Pure v_E (requires impl__is_err #v_T #v_E self) (fun _ -> Prims.l_True) =
   match self <: t_Result v_T v_E with
-  | Result_Ok t -> t
-  | Result_Err _ -> Core_models.Panicking.Internal.panic #v_T ()
+  | Result_Ok _ -> Core_models.Panicking.Internal.panic #v_E ()
+  | Result_Err e -> e
+
+/// See [`std::result::Result::unwrap_err`]
+let impl__unwrap_err (#v_T #v_E: Type0) (self: t_Result v_T v_E)
+    : Prims.Pure v_E (requires impl__is_err #v_T #v_E self) (fun _ -> Prims.l_True) =
+  match self <: t_Result v_T v_E with
+  | Result_Ok _ -> Core_models.Panicking.Internal.panic #v_E ()
+  | Result_Err e -> e
+
+/// See [`std::result::Result::cloned`]
+let impl_1__cloned
+      (#v_T #v_E: Type0)
+      (#[FStar.Tactics.Typeclasses.tcresolve ()] i0: Core_models.Clone.t_Clone v_T)
+      (self: t_Result v_T v_E)
+    : t_Result v_T v_E =
+  match self <: t_Result v_T v_E with
+  | Result_Ok t ->
+    Result_Ok (Core_models.Clone.f_clone #v_T #FStar.Tactics.Typeclasses.solve t)
+    <:
+    t_Result v_T v_E
+  | Result_Err e -> Result_Err e <: t_Result v_T v_E
+
+/// See [`std::result::Result::transpose`]
+let impl_2__transpose (#v_T #v_E: Type0) (self: t_Result (t_Option v_T) v_E)
+    : t_Option (t_Result v_T v_E) =
+  match self <: t_Result (t_Option v_T) v_E with
+  | Result_Ok (Option_Some t) ->
+    Option_Some (Result_Ok t <: t_Result v_T v_E) <: t_Option (t_Result v_T v_E)
+  | Result_Ok (Option_None ) -> Option_None <: t_Option (t_Result v_T v_E)
+  | Result_Err e -> Option_Some (Result_Err e <: t_Result v_T v_E) <: t_Option (t_Result v_T v_E)
+
+/// See [`std::result::Result::flatten`]
+let impl_3__flatten (#v_T #v_E: Type0) (self: t_Result (t_Result v_T v_E) v_E) : t_Result v_T v_E =
+  match self <: t_Result (t_Result v_T v_E) v_E with
+  | Result_Ok inner -> inner
+  | Result_Err e -> Result_Err e <: t_Result v_T v_E
