hax-lib/proof-libs/fstar/core/Alloc.Collections.Btree.Set.fst
@@ -1,0 +1,16 @@
+module Alloc.Collections.Btree.Set
+#set-options "--fuel 0 --ifuel 1 --z3rlimit 15"
+open FStar.Mul
+open Rust_primitives
+
+assume
+val t_BTreeSet': v_T: Type0 -> v_U: Type0 -> eqtype
+
+unfold
+let t_BTreeSet (v_T v_U: Type0) = t_BTreeSet' v_T v_U
+
+let impl_11__new (#v_T: Type0) (#v_U: Type0) (_: Prims.unit) : t_BTreeSet v_T v_U =
+  BTreeSet (Core_models.Option.Option_None <: Core_models.Option.t_Option v_T)
+    (Core_models.Option.Option_None <: Core_models.Option.t_Option v_U)
+  <:
+  t_BTreeSet v_T v_U
