hax-lib/proof-libs/fstar/core/Alloc.Slice.fst
@@ -3,14 +3,20 @@ module Alloc.Slice
 open FStar.Mul
 open Rust_primitives
 
-let impl__to_vec (#v_T: Type0) (s: t_Slice v_T) : Alloc.Vec.t_Vec v_T Alloc.Alloc.t_Global =
-  Alloc.Vec.Vec (Rust_primitives.Sequence.seq_from_slice #v_T s)
+let impl__to_vec
+      (#v_T: Type0)
+      (#[FStar.Tactics.Typeclasses.tcresolve ()] i0: Core_models.Clone.t_Clone v_T)
+      (s: t_Slice v_T)
+    : Alloc.Vec.t_Vec v_T Alloc.Alloc.t_Global =
+  let seq:Rust_primitives.Sequence.t_Seq v_T = Rust_primitives.Sequence.seq_empty #v_T () in
+  let seq:Rust_primitives.Sequence.t_Seq v_T = Rust_primitives.Sequence.seq_extend #v_T seq s in
+  Alloc.Vec.Vec seq
     (Core_models.Marker.PhantomData <: Core_models.Marker.t_PhantomData Alloc.Alloc.t_Global)
   <:
   Alloc.Vec.t_Vec v_T Alloc.Alloc.t_Global
 
 let impl__into_vec (#v_T #v_A: Type0) (s: t_Slice v_T) : Alloc.Vec.t_Vec v_T v_A =
-  Alloc.Vec.Vec (Rust_primitives.Sequence.seq_from_slice #v_T s)
+  Alloc.Vec.Vec (Rust_primitives.Sequence.seq_from_boxed_slice #v_T s)
     (Core_models.Marker.PhantomData <: Core_models.Marker.t_PhantomData v_A)
   <:
   Alloc.Vec.t_Vec v_T v_A
