hax-lib/proof-libs/fstar/core/Core_models.Iter.Adapters.Chain.fst
@@ -1,0 +1,10 @@
+module Core_models.Iter.Adapters.Chain
+#set-options "--fuel 0 --ifuel 1 --z3rlimit 15"
+open FStar.Mul
+open Rust_primitives
+
+include Core_models.Iter.Bundle {t_Chain as t_Chain}
+
+include Core_models.Iter.Bundle {impl__new as impl__new}
+
+include Core_models.Iter.Bundle {impl_1 as impl_1}
