hax-lib/proof-libs/fstar/core/Core_models.Ops.Bit.fsti
@@ -3,6 +3,51 @@ module Core_models.Ops.Bit
 open FStar.Mul
 open Rust_primitives
 
+/// See [`std::ops::ShrAssign`]
+class t_ShrAssign (v_Self: Type0) (v_Rhs: Type0) = {
+  f_shr_assign_pre:v_Self -> v_Rhs -> Type0;
+  f_shr_assign_post:v_Self -> v_Rhs -> v_Self -> Type0;
+  f_shr_assign:x0: v_Self -> x1: v_Rhs
+    -> Prims.Pure v_Self (f_shr_assign_pre x0 x1) (fun result -> f_shr_assign_post x0 x1 result)
+}
+
+/// See [`std::ops::ShlAssign`]
+class t_ShlAssign (v_Self: Type0) (v_Rhs: Type0) = {
+  f_shl_assign_pre:v_Self -> v_Rhs -> Type0;
+  f_shl_assign_post:v_Self -> v_Rhs -> v_Self -> Type0;
+  f_shl_assign:x0: v_Self -> x1: v_Rhs
+    -> Prims.Pure v_Self (f_shl_assign_pre x0 x1) (fun result -> f_shl_assign_post x0 x1 result)
+}
+
+/// See [`std::ops::BitXorAssign`]
+class t_BitXorAssign (v_Self: Type0) (v_Rhs: Type0) = {
+  f_bitxor_assign_pre:v_Self -> v_Rhs -> Type0;
+  f_bitxor_assign_post:v_Self -> v_Rhs -> v_Self -> Type0;
+  f_bitxor_assign:x0: v_Self -> x1: v_Rhs
+    -> Prims.Pure v_Self
+        (f_bitxor_assign_pre x0 x1)
+        (fun result -> f_bitxor_assign_post x0 x1 result)
+}
+
+/// See [`std::ops::BitAndAssign`]
+class t_BitAndAssign (v_Self: Type0) (v_Rhs: Type0) = {
+  f_bitand_assign_pre:v_Self -> v_Rhs -> Type0;
+  f_bitand_assign_post:v_Self -> v_Rhs -> v_Self -> Type0;
+  f_bitand_assign:x0: v_Self -> x1: v_Rhs
+    -> Prims.Pure v_Self
+        (f_bitand_assign_pre x0 x1)
+        (fun result -> f_bitand_assign_post x0 x1 result)
+}
+
+/// See [`std::ops::BitOrAssign`]
+class t_BitOrAssign (v_Self: Type0) (v_Rhs: Type0) = {
+  f_bitor_assign_pre:v_Self -> v_Rhs -> Type0;
+  f_bitor_assign_post:v_Self -> v_Rhs -> v_Self -> Type0;
+  f_bitor_assign:x0: v_Self -> x1: v_Rhs
+    -> Prims.Pure v_Self (f_bitor_assign_pre x0 x1) (fun result -> f_bitor_assign_post x0 x1 result)
+}
+
+/// See [`std::ops::Shr`]
 class t_Shr (v_Self: Type0) (v_Rhs: Type0) = {
   [@@@ FStar.Tactics.Typeclasses.no_method]f_Output:Type0;
   f_shr_pre:v_Self -> v_Rhs -> Type0;
@@ -11,6 +56,7 @@ class t_Shr (v_Self: Type0) (v_Rhs: Type0) = {
     -> Prims.Pure f_Output (f_shr_pre x0 x1) (fun result -> f_shr_post x0 x1 result)
 }
 
+/// See [`std::ops::Shl`]
 class t_Shl (v_Self: Type0) (v_Rhs: Type0) = {
   [@@@ FStar.Tactics.Typeclasses.no_method]f_Output:Type0;
   f_shl_pre:v_Self -> v_Rhs -> Type0;
@@ -19,6 +65,7 @@ class t_Shl (v_Self: Type0) (v_Rhs: Type0) = {
     -> Prims.Pure f_Output (f_shl_pre x0 x1) (fun result -> f_shl_post x0 x1 result)
 }
 
+/// See [`std::ops::BitXor`]
 class t_BitXor (v_Self: Type0) (v_Rhs: Type0) = {
   [@@@ FStar.Tactics.Typeclasses.no_method]f_Output:Type0;
   f_bitxor_pre:v_Self -> v_Rhs -> Type0;
@@ -27,6 +74,7 @@ class t_BitXor (v_Self: Type0) (v_Rhs: Type0) = {
     -> Prims.Pure f_Output (f_bitxor_pre x0 x1) (fun result -> f_bitxor_post x0 x1 result)
 }
 
+/// See [`std::ops::BitAnd`]
 class t_BitAnd (v_Self: Type0) (v_Rhs: Type0) = {
   [@@@ FStar.Tactics.Typeclasses.no_method]f_Output:Type0;
   f_bitand_pre:v_Self -> v_Rhs -> Type0;
@@ -35,10 +83,19 @@ class t_BitAnd (v_Self: Type0) (v_Rhs: Type0) = {
     -> Prims.Pure f_Output (f_bitand_pre x0 x1) (fun result -> f_bitand_post x0 x1 result)
 }
 
+/// See [`std::ops::BitOr`]
 class t_BitOr (v_Self: Type0) (v_Rhs: Type0) = {
   [@@@ FStar.Tactics.Typeclasses.no_method]f_Output:Type0;
   f_bitor_pre:v_Self -> v_Rhs -> Type0;
   f_bitor_post:v_Self -> v_Rhs -> f_Output -> Type0;
   f_bitor:x0: v_Self -> x1: v_Rhs
     -> Prims.Pure f_Output (f_bitor_pre x0 x1) (fun result -> f_bitor_post x0 x1 result)
+}
+
+/// See [`std::ops::Not`]
+class t_Not (v_Self: Type0) = {
+  [@@@ FStar.Tactics.Typeclasses.no_method]f_Output:Type0;
+  f_not_pre:v_Self -> Type0;
+  f_not_post:v_Self -> f_Output -> Type0;
+  f_not:x0: v_Self -> Prims.Pure f_Output (f_not_pre x0) (fun result -> f_not_post x0 result)
 }
