hax-lib/proof-libs/fstar/core/Core_models.Ops.Function.fst
@@ -3,6 +3,7 @@ module Core_models.Ops.Function
 open FStar.Mul
 open Rust_primitives
 
+/// See [`std::ops::FnOnce`]
 class t_FnOnce (v_Self: Type0) (v_Args: Type0) = {
   [@@@ FStar.Tactics.Typeclasses.no_method]f_Output:Type0;
   f_call_once_pre:self_: v_Self -> args: v_Args -> pred: Type0{true ==> pred};
@@ -11,19 +12,36 @@ class t_FnOnce (v_Self: Type0) (v_Args: Type0) = {
     -> Prims.Pure f_Output (f_call_once_pre x0 x1) (fun result -> f_call_once_post x0 x1 result)
 }
 
-class t_Fn (v_Self: Type0) (v_Args: Type0) = {
+/// See [`std::ops::Fn`]
+class t_FnMut (v_Self: Type0) (v_Args: Type0) = {
   [@@@ FStar.Tactics.Typeclasses.no_method]_super_i0:t_FnOnce v_Self v_Args;
+  f_call_mut_pre:self_: v_Self -> args: v_Args -> pred: Type0{true ==> pred};
+  f_call_mut_post:v_Self -> v_Args -> (_super_i0).f_Output -> Type0;
+  f_call_mut:x0: v_Self -> x1: v_Args
+    -> Prims.Pure (_super_i0).f_Output
+        (f_call_mut_pre x0 x1)
+        (fun result -> f_call_mut_post x0 x1 result)
+}
+
+[@@ FStar.Tactics.Typeclasses.tcinstance]
+let _ = fun (v_Self:Type0) (v_Args:Type0) {|i: t_FnMut v_Self v_Args|} -> i._super_i0
+
+/// See [`std::ops::Fn`]
+class t_Fn (v_Self: Type0) (v_Args: Type0) = {
+  [@@@ FStar.Tactics.Typeclasses.no_method]_super_i0:t_FnMut v_Self v_Args;
   f_call_pre:self_: v_Self -> args: v_Args -> pred: Type0{true ==> pred};
-  f_call_post:v_Self -> v_Args -> (_super_i0).f_Output -> Type0;
+  f_call_post:v_Self -> v_Args -> (_super_i0)._super_i0.f_Output -> Type0;
   f_call:x0: v_Self -> x1: v_Args
-    -> Prims.Pure (_super_i0).f_Output (f_call_pre x0 x1) (fun result -> f_call_post x0 x1 result)
+    -> Prims.Pure (_super_i0)._super_i0.f_Output
+        (f_call_pre x0 x1)
+        (fun result -> f_call_post x0 x1 result)
 }
 
 [@@ FStar.Tactics.Typeclasses.tcinstance]
 let _ = fun (v_Self:Type0) (v_Args:Type0) {|i: t_Fn v_Self v_Args|} -> i._super_i0
 
 [@@ FStar.Tactics.Typeclasses.tcinstance]
-let impl_2 (#v_Arg #v_Out: Type0) : t_FnOnce (v_Arg -> v_Out) v_Arg =
+let impl_6 (#v_Arg #v_Out: Type0) : t_FnOnce (v_Arg -> v_Out) v_Arg =
   {
     f_Output = v_Out;
     f_call_once_pre = (fun (self: (v_Arg -> v_Out)) (arg: v_Arg) -> true);
@@ -69,6 +87,108 @@ let impl_1 (#v_Arg1 #v_Arg2 #v_Arg3 #v_Out: Type0)
         ->
         true);
     f_call_once
+    =
+    fun (self: (v_Arg1 -> v_Arg2 -> v_Arg3 -> v_Out)) (arg: (v_Arg1 & v_Arg2 & v_Arg3)) ->
+      self arg._1 arg._2 arg._3
+  }
+
+[@@ FStar.Tactics.Typeclasses.tcinstance]
+let impl_7 (#v_Arg #v_Out: Type0) : t_FnMut (v_Arg -> v_Out) v_Arg =
+  {
+    _super_i0 = FStar.Tactics.Typeclasses.solve;
+    f_call_mut_pre = (fun (self: (v_Arg -> v_Out)) (arg: v_Arg) -> true);
+    f_call_mut_post = (fun (self: (v_Arg -> v_Out)) (arg: v_Arg) (out: v_Out) -> true);
+    f_call_mut = fun (self: (v_Arg -> v_Out)) (arg: v_Arg) -> self arg
+  }
+
+unfold instance fnmut_arrow_binder t u
+  : t_FnMut (_:t -> u) t = {
+    f_Output = u;
+    f_call_mut_pre = (fun _ _ -> true);
+    f_call_mut_post = (fun (x0: (_:t -> u)) (x1: t) (res: u) -> res == x0 x1);
+    f_call_mut = (fun (x0: (_:t -> u)) (x1: t) -> x0 x1);
+  }
+
+[@@ FStar.Tactics.Typeclasses.tcinstance]
+let impl_2 (#v_Arg1 #v_Arg2 #v_Out: Type0) : t_FnMut (v_Arg1 -> v_Arg2 -> v_Out) (v_Arg1 & v_Arg2) =
+  {
+    _super_i0 = FStar.Tactics.Typeclasses.solve;
+    f_call_mut_pre = (fun (self: (v_Arg1 -> v_Arg2 -> v_Out)) (arg: (v_Arg1 & v_Arg2)) -> true);
+    f_call_mut_post
+    =
+    (fun (self: (v_Arg1 -> v_Arg2 -> v_Out)) (arg: (v_Arg1 & v_Arg2)) (out: v_Out) -> true);
+    f_call_mut
+    =
+    fun (self: (v_Arg1 -> v_Arg2 -> v_Out)) (arg: (v_Arg1 & v_Arg2)) -> self arg._1 arg._2
+  }
+
+[@@ FStar.Tactics.Typeclasses.tcinstance]
+let impl_3 (#v_Arg1 #v_Arg2 #v_Arg3 #v_Out: Type0)
+    : t_FnMut (v_Arg1 -> v_Arg2 -> v_Arg3 -> v_Out) (v_Arg1 & v_Arg2 & v_Arg3) =
+  {
+    _super_i0 = FStar.Tactics.Typeclasses.solve;
+    f_call_mut_pre
+    =
+    (fun (self: (v_Arg1 -> v_Arg2 -> v_Arg3 -> v_Out)) (arg: (v_Arg1 & v_Arg2 & v_Arg3)) -> true);
+    f_call_mut_post
+    =
+    (fun
+        (self: (v_Arg1 -> v_Arg2 -> v_Arg3 -> v_Out))
+        (arg: (v_Arg1 & v_Arg2 & v_Arg3))
+        (out: v_Out)
+        ->
+        true);
+    f_call_mut
+    =
+    fun (self: (v_Arg1 -> v_Arg2 -> v_Arg3 -> v_Out)) (arg: (v_Arg1 & v_Arg2 & v_Arg3)) ->
+      self arg._1 arg._2 arg._3
+  }
+
+[@@ FStar.Tactics.Typeclasses.tcinstance]
+let impl_8 (#v_Arg #v_Out: Type0) : t_Fn (v_Arg -> v_Out) v_Arg =
+  {
+    _super_i0 = FStar.Tactics.Typeclasses.solve;
+    f_call_pre = (fun (self: (v_Arg -> v_Out)) (arg: v_Arg) -> true);
+    f_call_post = (fun (self: (v_Arg -> v_Out)) (arg: v_Arg) (out: v_Out) -> true);
+    f_call = fun (self: (v_Arg -> v_Out)) (arg: v_Arg) -> self arg
+  }
+
+unfold instance fn_arrow_binder t u
+  : t_Fn (_:t -> u) t = {
+    f_Output = u;
+    f_call_pre = (fun _ _ -> true);
+    f_call_post = (fun (x0: (_:t -> u)) (x1: t) (res: u) -> res == x0 x1);
+    f_call = (fun (x0: (_:t -> u)) (x1: t) -> x0 x1);
+  }
+
+[@@ FStar.Tactics.Typeclasses.tcinstance]
+let impl_4 (#v_Arg1 #v_Arg2 #v_Out: Type0) : t_Fn (v_Arg1 -> v_Arg2 -> v_Out) (v_Arg1 & v_Arg2) =
+  {
+    _super_i0 = FStar.Tactics.Typeclasses.solve;
+    f_call_pre = (fun (self: (v_Arg1 -> v_Arg2 -> v_Out)) (arg: (v_Arg1 & v_Arg2)) -> true);
+    f_call_post
+    =
+    (fun (self: (v_Arg1 -> v_Arg2 -> v_Out)) (arg: (v_Arg1 & v_Arg2)) (out: v_Out) -> true);
+    f_call = fun (self: (v_Arg1 -> v_Arg2 -> v_Out)) (arg: (v_Arg1 & v_Arg2)) -> self arg._1 arg._2
+  }
+
+[@@ FStar.Tactics.Typeclasses.tcinstance]
+let impl_5 (#v_Arg1 #v_Arg2 #v_Arg3 #v_Out: Type0)
+    : t_Fn (v_Arg1 -> v_Arg2 -> v_Arg3 -> v_Out) (v_Arg1 & v_Arg2 & v_Arg3) =
+  {
+    _super_i0 = FStar.Tactics.Typeclasses.solve;
+    f_call_pre
+    =
+    (fun (self: (v_Arg1 -> v_Arg2 -> v_Arg3 -> v_Out)) (arg: (v_Arg1 & v_Arg2 & v_Arg3)) -> true);
+    f_call_post
+    =
+    (fun
+        (self: (v_Arg1 -> v_Arg2 -> v_Arg3 -> v_Out))
+        (arg: (v_Arg1 & v_Arg2 & v_Arg3))
+        (out: v_Out)
+        ->
+        true);
+    f_call
     =
     fun (self: (v_Arg1 -> v_Arg2 -> v_Arg3 -> v_Out)) (arg: (v_Arg1 & v_Arg2 & v_Arg3)) ->
       self arg._1 arg._2 arg._3
