hax-lib/proof-libs/fstar/core/Core_models.Slice.fst
@@ -3,27 +3,42 @@ module Core_models.Slice
 open FStar.Mul
 open Rust_primitives
 
+/// See [`std::slice::len`]
 let impl__len (#v_T: Type0) (s: t_Slice v_T) : usize = Rust_primitives.Slice.slice_length #v_T s
 
+/// See [`std::slice::chunks`]
 let impl__chunks (#v_T: Type0) (s: t_Slice v_T) (cs: usize) : Core_models.Slice.Iter.t_Chunks v_T =
   Core_models.Slice.Iter.impl__new #v_T cs s
 
+/// See [`std::slice::iter`]
 let impl__iter (#v_T: Type0) (s: t_Slice v_T) : Core_models.Slice.Iter.t_Iter v_T =
   Core_models.Slice.Iter.Iter (Rust_primitives.Sequence.seq_from_slice #v_T s)
   <:
   Core_models.Slice.Iter.t_Iter v_T
 
+/// See [`std::slice::chunks_exact`]
 let impl__chunks_exact (#v_T: Type0) (s: t_Slice v_T) (cs: usize)
     : Core_models.Slice.Iter.t_ChunksExact v_T = Core_models.Slice.Iter.impl_1__new #v_T cs s
 
+/// See [`std::slice::is_empty`]
 let impl__is_empty (#v_T: Type0) (s: t_Slice v_T) : bool = (impl__len #v_T s <: usize) =. mk_usize 0
 
+/// See [`std::slice::contains`]
 assume
-val impl__contains': #v_T: Type0 -> s: t_Slice v_T -> v: v_T -> bool
+val impl__contains':
+    #v_T: Type0 ->
+    {| i0: Core_models.Cmp.t_PartialEq v_T v_T |} ->
+    s: t_Slice v_T ->
+    v: v_T
+  -> bool
 
 unfold
-let impl__contains (#v_T: Type0) = impl__contains' #v_T
+let impl__contains
+      (#v_T: Type0)
+      (#[FStar.Tactics.Typeclasses.tcresolve ()] i0: Core_models.Cmp.t_PartialEq v_T v_T)
+     = impl__contains' #v_T #i0
 
+/// See [`std::slice::copy_within`]
 assume
 val impl__copy_within':
     #v_T: Type0 ->
@@ -40,6 +55,7 @@ let impl__copy_within
       (#[FStar.Tactics.Typeclasses.tcresolve ()] i0: Core_models.Marker.t_Copy v_T)
      = impl__copy_within' #v_T #v_R #i0
 
+/// See [`std::slice::binary_search`]
 assume
 val impl__binary_search': #v_T: Type0 -> s: t_Slice v_T -> x: v_T
   -> Core_models.Result.t_Result usize usize
@@ -47,6 +63,89 @@ val impl__binary_search': #v_T: Type0 -> s: t_Slice v_T -> x: v_T
 unfold
 let impl__binary_search (#v_T: Type0) = impl__binary_search' #v_T
 
+/// See [`std::slice::get`]
+let impl__get
+      (#v_T #v_I: Type0)
+      (#[FStar.Tactics.Typeclasses.tcresolve ()]
+          i0:
+          Core_models.Slice.Index.t_SliceIndex v_I (t_Slice v_T))
+      (s: t_Slice v_T)
+      (index: v_I)
+    : Core_models.Option.t_Option i0.f_Output =
+  Core_models.Slice.Index.f_get #v_I #(t_Slice v_T) #FStar.Tactics.Typeclasses.solve index s
+
+/// See [`std::slice::first`]
+let impl__first (#v_T: Type0) (s: t_Slice v_T) : Core_models.Option.t_Option v_T =
+  if impl__is_empty #v_T s
+  then Core_models.Option.Option_None <: Core_models.Option.t_Option v_T
+  else
+    Core_models.Option.Option_Some (Rust_primitives.Slice.slice_index #v_T s (mk_usize 0))
+    <:
+    Core_models.Option.t_Option v_T
+
+/// See [`std::slice::last`]
+let impl__last (#v_T: Type0) (s: t_Slice v_T) : Core_models.Option.t_Option v_T =
+  if impl__is_empty #v_T s
+  then Core_models.Option.Option_None <: Core_models.Option.t_Option v_T
+  else
+    Core_models.Option.Option_Some
+    (Rust_primitives.Slice.slice_index #v_T s ((impl__len #v_T s <: usize) -! mk_usize 1 <: usize))
+    <:
+    Core_models.Option.t_Option v_T
+
+/// See [`std::slice::reverse`]
+assume
+val impl__reverse': #v_T: Type0 -> s: t_Slice v_T -> t_Slice v_T
+
+unfold
+let impl__reverse (#v_T: Type0) = impl__reverse' #v_T
+
+/// See [`std::slice::starts_with`]
+assume
+val impl__starts_with':
+    #v_T: Type0 ->
+    {| i0: Core_models.Cmp.t_PartialEq v_T v_T |} ->
+    s: t_Slice v_T ->
+    needle: t_Slice v_T
+  -> bool
+
+unfold
+let impl__starts_with
+      (#v_T: Type0)
+      (#[FStar.Tactics.Typeclasses.tcresolve ()] i0: Core_models.Cmp.t_PartialEq v_T v_T)
+     = impl__starts_with' #v_T #i0
+
+/// See [`std::slice::ends_with`]
+assume
+val impl__ends_with':
+    #v_T: Type0 ->
+    {| i0: Core_models.Cmp.t_PartialEq v_T v_T |} ->
+    s: t_Slice v_T ->
+    needle: t_Slice v_T
+  -> bool
+
+unfold
+let impl__ends_with
+      (#v_T: Type0)
+      (#[FStar.Tactics.Typeclasses.tcresolve ()] i0: Core_models.Cmp.t_PartialEq v_T v_T)
+     = impl__ends_with' #v_T #i0
+
+/// See [`std::slice::fill`]
+assume
+val impl__fill':
+    #v_T: Type0 ->
+    {| i0: Core_models.Clone.t_Clone v_T |} ->
+    s: t_Slice v_T ->
+    value: v_T
+  -> t_Slice v_T
+
+unfold
+let impl__fill
+      (#v_T: Type0)
+      (#[FStar.Tactics.Typeclasses.tcresolve ()] i0: Core_models.Clone.t_Clone v_T)
+     = impl__fill' #v_T #i0
+
+/// See [`std::slice::copy_from_slice`]
 let impl__copy_from_slice
       (#v_T: Type0)
       (#[FStar.Tactics.Typeclasses.tcresolve ()] i0: Core_models.Marker.t_Copy v_T)
@@ -54,11 +153,10 @@ let impl__copy_from_slice
     : Prims.Pure (t_Slice v_T)
       (requires (impl__len #v_T s <: usize) =. (impl__len #v_T src <: usize))
       (fun _ -> Prims.l_True) =
-  let (tmp0: t_Slice v_T), (out: t_Slice v_T) = Rust_primitives.Mem.replace #(t_Slice v_T) s src in
-  let s:t_Slice v_T = tmp0 in
-  let _:t_Slice v_T = out in
+  let s:t_Slice v_T = Rust_primitives.Slice.slice_clone_from_slice #v_T s src in
   s
 
+/// See [`std::slice::clone_from_slice`]
 let impl__clone_from_slice
       (#v_T: Type0)
       (#[FStar.Tactics.Typeclasses.tcresolve ()] i0: Core_models.Clone.t_Clone v_T)
@@ -66,16 +164,16 @@ let impl__clone_from_slice
     : Prims.Pure (t_Slice v_T)
       (requires (impl__len #v_T s <: usize) =. (impl__len #v_T src <: usize))
       (fun _ -> Prims.l_True) =
-  let (tmp0: t_Slice v_T), (out: t_Slice v_T) = Rust_primitives.Mem.replace #(t_Slice v_T) s src in
-  let s:t_Slice v_T = tmp0 in
-  let _:t_Slice v_T = out in
+  let s:t_Slice v_T = Rust_primitives.Slice.slice_clone_from_slice #v_T s src in
   s
 
+/// See [`std::slice::split_at`]
 let impl__split_at (#v_T: Type0) (s: t_Slice v_T) (mid: usize)
     : Prims.Pure (t_Slice v_T & t_Slice v_T)
       (requires mid <=. (impl__len #v_T s <: usize))
       (fun _ -> Prims.l_True) = Rust_primitives.Slice.slice_split_at #v_T s mid
 
+/// See [`std::slice::split_at_checked`]
 let impl__split_at_checked (#v_T: Type0) (s: t_Slice v_T) (mid: usize)
     : Core_models.Option.t_Option (t_Slice v_T & t_Slice v_T) =
   if mid <=. (impl__len #v_T s <: usize)
@@ -85,9 +183,30 @@ let impl__split_at_checked (#v_T: Type0) (s: t_Slice v_T) (mid: usize)
     Core_models.Option.t_Option (t_Slice v_T & t_Slice v_T)
   else Core_models.Option.Option_None <: Core_models.Option.t_Option (t_Slice v_T & t_Slice v_T)
 
+/// See [`std::slice::swap`]
+assume
+val impl__swap': #v_T: Type0 -> s: t_Slice v_T -> a: usize -> b: usize
+  -> Prims.Pure (t_Slice v_T)
+      (requires a <. (impl__len #v_T s <: usize) && b <. (impl__len #v_T s <: usize))
+      (fun _ -> Prims.l_True)
+
+unfold
+let impl__swap (#v_T: Type0) = impl__swap' #v_T
+
+/// See [`std::slice::windows`]
+let impl__windows (#v_T: Type0) (s: t_Slice v_T) (size: usize)
+    : Prims.Pure (Core_models.Slice.Iter.t_Windows v_T)
+      (requires size >. mk_usize 0)
+      (fun _ -> Prims.l_True) =
+  let _:Prims.unit =
+    if size =. mk_usize 0 then Core_models.Panicking.Internal.panic #Prims.unit ()
+  in
+  Core_models.Slice.Iter.impl_5__new #v_T size s
+
 [@@ FStar.Tactics.Typeclasses.tcinstance]
 let impl_1 (#v_T: Type0) : Core_models.Iter.Traits.Collect.t_IntoIterator (t_Slice v_T) =
   {
+    f_Item = v_T;
     f_IntoIter = Core_models.Slice.Iter.t_Iter v_T;
     f_into_iter_pre = (fun (self: t_Slice v_T) -> true);
     f_into_iter_post = (fun (self: t_Slice v_T) (out: Core_models.Slice.Iter.t_Iter v_T) -> true);
@@ -95,7 +214,7 @@ let impl_1 (#v_T: Type0) : Core_models.Iter.Traits.Collect.t_IntoIterator (t_Sli
   }
 
 [@@ FStar.Tactics.Typeclasses.tcinstance]
-let impl_7 (#v_T: Type0)
+let impl_2 (#v_T: Type0)
     : Core_models.Ops.Index.t_Index (t_Slice v_T) (Core_models.Ops.Range.t_Range usize) =
   {
     f_Output = t_Slice v_T;
@@ -117,7 +236,7 @@ let impl_7 (#v_T: Type0)
   }
 
 [@@ FStar.Tactics.Typeclasses.tcinstance]
-let impl_8 (#v_T: Type0)
+let impl_3 (#v_T: Type0)
     : Core_models.Ops.Index.t_Index (t_Slice v_T) (Core_models.Ops.Range.t_RangeTo usize) =
   {
     f_Output = t_Slice v_T;
@@ -135,7 +254,7 @@ let impl_8 (#v_T: Type0)
   }
 
 [@@ FStar.Tactics.Typeclasses.tcinstance]
-let impl_9 (#v_T: Type0)
+let impl_4 (#v_T: Type0)
     : Core_models.Ops.Index.t_Index (t_Slice v_T) (Core_models.Ops.Range.t_RangeFrom usize) =
   {
     f_Output = t_Slice v_T;
@@ -157,7 +276,7 @@ let impl_9 (#v_T: Type0)
   }
 
 [@@ FStar.Tactics.Typeclasses.tcinstance]
-let impl_10 (#v_T: Type0)
+let impl_5 (#v_T: Type0)
     : Core_models.Ops.Index.t_Index (t_Slice v_T) Core_models.Ops.Range.t_RangeFull =
   {
     f_Output = t_Slice v_T;
@@ -175,149 +294,10 @@ let impl_10 (#v_T: Type0)
   }
 
 [@@ FStar.Tactics.Typeclasses.tcinstance]
-let impl_11 (#v_T: Type0) : Core_models.Ops.Index.t_Index (t_Slice v_T) usize =
+let impl_6 (#v_T: Type0) : Core_models.Ops.Index.t_Index (t_Slice v_T) usize =
   {
     f_Output = v_T;
     f_index_pre = (fun (self_: t_Slice v_T) (i: usize) -> i <. (impl__len #v_T self_ <: usize));
     f_index_post = (fun (self: t_Slice v_T) (i: usize) (out: v_T) -> true);
     f_index = fun (self: t_Slice v_T) (i: usize) -> Rust_primitives.Slice.slice_index #v_T self i
-  }
-
-class t_SliceIndex (v_Self: Type0) (v_T: Type0) = {
-  [@@@ FStar.Tactics.Typeclasses.no_method]f_Output:Type0;
-  f_get_pre:self_: v_Self -> slice: v_T -> pred: Type0{true ==> pred};
-  f_get_post:v_Self -> v_T -> Core_models.Option.t_Option f_Output -> Type0;
-  f_get:x0: v_Self -> x1: v_T
-    -> Prims.Pure (Core_models.Option.t_Option f_Output)
-        (f_get_pre x0 x1)
-        (fun result -> f_get_post x0 x1 result)
-}
-
-let impl__get
-      (#v_T #v_I: Type0)
-      (#[FStar.Tactics.Typeclasses.tcresolve ()] i0: t_SliceIndex v_I (t_Slice v_T))
-      (s: t_Slice v_T)
-      (index: v_I)
-    : Core_models.Option.t_Option i0.f_Output =
-  f_get #v_I #(t_Slice v_T) #FStar.Tactics.Typeclasses.solve index s
-
-[@@ FStar.Tactics.Typeclasses.tcinstance]
-let impl_2 (#v_T: Type0) : t_SliceIndex usize (t_Slice v_T) =
-  {
-    f_Output = v_T;
-    f_get_pre = (fun (self: usize) (slice: t_Slice v_T) -> true);
-    f_get_post
-    =
-    (fun (self: usize) (slice: t_Slice v_T) (out: Core_models.Option.t_Option v_T) -> true);
-    f_get
-    =
-    fun (self: usize) (slice: t_Slice v_T) ->
-      if self <. (impl__len #v_T slice <: usize)
-      then
-        Core_models.Option.Option_Some (Rust_primitives.Slice.slice_index #v_T slice self)
-        <:
-        Core_models.Option.t_Option v_T
-      else Core_models.Option.Option_None <: Core_models.Option.t_Option v_T
-  }
-
-[@@ FStar.Tactics.Typeclasses.tcinstance]
-let impl_3 (#v_T: Type0) : t_SliceIndex Core_models.Ops.Range.t_RangeFull (t_Slice v_T) =
-  {
-    f_Output = t_Slice v_T;
-    f_get_pre = (fun (self: Core_models.Ops.Range.t_RangeFull) (slice: t_Slice v_T) -> true);
-    f_get_post
-    =
-    (fun
-        (self: Core_models.Ops.Range.t_RangeFull)
-        (slice: t_Slice v_T)
-        (out: Core_models.Option.t_Option (t_Slice v_T))
-        ->
-        true);
-    f_get
-    =
-    fun (self: Core_models.Ops.Range.t_RangeFull) (slice: t_Slice v_T) ->
-      Core_models.Option.Option_Some slice <: Core_models.Option.t_Option (t_Slice v_T)
-  }
-
-[@@ FStar.Tactics.Typeclasses.tcinstance]
-let impl_4 (#v_T: Type0) : t_SliceIndex (Core_models.Ops.Range.t_RangeFrom usize) (t_Slice v_T) =
-  {
-    f_Output = t_Slice v_T;
-    f_get_pre = (fun (self: Core_models.Ops.Range.t_RangeFrom usize) (slice: t_Slice v_T) -> true);
-    f_get_post
-    =
-    (fun
-        (self: Core_models.Ops.Range.t_RangeFrom usize)
-        (slice: t_Slice v_T)
-        (out: Core_models.Option.t_Option (t_Slice v_T))
-        ->
-        true);
-    f_get
-    =
-    fun (self: Core_models.Ops.Range.t_RangeFrom usize) (slice: t_Slice v_T) ->
-      if self.Core_models.Ops.Range.f_start <. (impl__len #v_T slice <: usize)
-      then
-        Core_models.Option.Option_Some
-        (Rust_primitives.Slice.slice_slice #v_T
-            slice
-            self.Core_models.Ops.Range.f_start
-            (impl__len #v_T slice <: usize))
-        <:
-        Core_models.Option.t_Option (t_Slice v_T)
-      else Core_models.Option.Option_None <: Core_models.Option.t_Option (t_Slice v_T)
-  }
-
-[@@ FStar.Tactics.Typeclasses.tcinstance]
-let impl_5 (#v_T: Type0) : t_SliceIndex (Core_models.Ops.Range.t_RangeTo usize) (t_Slice v_T) =
-  {
-    f_Output = t_Slice v_T;
-    f_get_pre = (fun (self: Core_models.Ops.Range.t_RangeTo usize) (slice: t_Slice v_T) -> true);
-    f_get_post
-    =
-    (fun
-        (self: Core_models.Ops.Range.t_RangeTo usize)
-        (slice: t_Slice v_T)
-        (out: Core_models.Option.t_Option (t_Slice v_T))
-        ->
-        true);
-    f_get
-    =
-    fun (self: Core_models.Ops.Range.t_RangeTo usize) (slice: t_Slice v_T) ->
-      if self.Core_models.Ops.Range.f_end <=. (impl__len #v_T slice <: usize)
-      then
-        Core_models.Option.Option_Some
-        (Rust_primitives.Slice.slice_slice #v_T slice (mk_usize 0) self.Core_models.Ops.Range.f_end)
-        <:
-        Core_models.Option.t_Option (t_Slice v_T)
-      else Core_models.Option.Option_None <: Core_models.Option.t_Option (t_Slice v_T)
-  }
-
-[@@ FStar.Tactics.Typeclasses.tcinstance]
-let impl_6 (#v_T: Type0) : t_SliceIndex (Core_models.Ops.Range.t_Range usize) (t_Slice v_T) =
-  {
-    f_Output = t_Slice v_T;
-    f_get_pre = (fun (self: Core_models.Ops.Range.t_Range usize) (slice: t_Slice v_T) -> true);
-    f_get_post
-    =
-    (fun
-        (self: Core_models.Ops.Range.t_Range usize)
-        (slice: t_Slice v_T)
-        (out: Core_models.Option.t_Option (t_Slice v_T))
-        ->
-        true);
-    f_get
-    =
-    fun (self: Core_models.Ops.Range.t_Range usize) (slice: t_Slice v_T) ->
-      if
-        self.Core_models.Ops.Range.f_start <. self.Core_models.Ops.Range.f_end &&
-        self.Core_models.Ops.Range.f_end <=. (impl__len #v_T slice <: usize)
-      then
-        Core_models.Option.Option_Some
-        (Rust_primitives.Slice.slice_slice #v_T
-            slice
-            self.Core_models.Ops.Range.f_start
-            self.Core_models.Ops.Range.f_end)
-        <:
-        Core_models.Option.t_Option (t_Slice v_T)
-      else Core_models.Option.Option_None <: Core_models.Option.t_Option (t_Slice v_T)
   }
